theories/examples/stack_macros.v
@@ -1,8 +1,8 @@
 From iris.algebra Require Import frac.
 From iris.proofmode Require Import tactics.
 Require Import Eqdep_dec List.
-From cap_machine Require Import rules logrel fundamental monotone. 
-From cap_machine Require Export contiguous region_macros.
+From cap_machine Require Import rules logrel fundamental monotone.
+From cap_machine Require Export addr_reg_sample region_macros contiguous.
 
 Section stack_macros.
   Context `{memG Σ, regG Σ, STSG Σ, logrel_na_invs Σ,
@@ -15,7 +15,7 @@ Section stack_macros.
     isCorrectPC (inr (p, g, b, e, a0))
     → isCorrectPC (inr (p, g, b, e, a2))
     → (a0 ≤ a1)%Z ∧ (a1 ≤ a2)%Z
-    → isCorrectPC (inr (p, g, b, e, a1)). 
+    → isCorrectPC (inr (p, g, b, e, a1)).
   Proof.
     intros Hvpc0 Hvpc2 [Hle0 Hle2].
     apply Z.lt_eq_cases in Hle2 as [Hlt2 | Heq2].
@@ -33,11 +33,69 @@ Section stack_macros.
     rewrite /withinBounds.
     apply andb_true_iff.
     apply andb_true_iff in Hwb0 as [Hleb0 Hlea0].
-    apply andb_true_iff in Hwb2 as [Hleb2 Hlea2].  
-    split; rewrite /leb_addr; apply Z.leb_le.
-    - apply Z.leb_le in Hleb0. apply Z.leb_le in Hlea0. lia.
-    - apply Z.leb_le in Hleb2. apply Z.leb_le in Hlea2. lia.
-  Qed. 
+    apply andb_true_iff in Hwb2 as [Hleb2 Hlea2].
+    split; rewrite /leb_addr /ltb_addr; first [ apply Z.leb_le | apply Z.ltb_lt ].
+    - apply Z.leb_le in Hleb0. apply Z.ltb_lt in Hlea0. lia.
+    - apply Z.leb_le in Hleb2. apply Z.ltb_lt in Hlea2. lia.
+  Qed.
+
+  Lemma isWithinBounds_bounds_alt' p g b e (a0 a1 a2 : Addr) :
+    withinBounds (p,g,b,e,a0) = true ->
+    withinBounds (p,g,b,e,a2) = true ->
+    (a0 ≤ a1)%Z ∧ (a1 < a2)%Z ->
+    withinBounds (p,g,b,e,a1) = true.
+  Proof.
+    intros Hwb0 Hwb2 [Hle0 Hle2].
+    rewrite /withinBounds.
+    apply andb_true_iff.
+    apply andb_true_iff in Hwb0 as [Hleb0 Hlea0].
+    apply andb_true_iff in Hwb2 as [Hleb2 Hlea2].
+    split; rewrite /leb_addr /ltb_addr; first [ apply Z.leb_le | apply Z.ltb_lt ].
+    - apply Z.leb_le in Hleb0. apply Z.ltb_lt in Hlea0. lia.
+    - apply Z.leb_le in Hleb2. apply Z.ltb_lt in Hlea2. lia.
+  Qed.
+
+  Definition isCorrectPC_range p g b e a0 an :=
+    ∀ ai, (a0 <= ai)%a ∧ (ai < an)%a → isCorrectPC (inr (p, g, b, e, ai)).
+
+  Lemma isCorrectPC_inrange p g b (e a0 an a: Addr) :
+    isCorrectPC_range p g b e a0 an →
+    (a0 <= a < an)%Z →
+    isCorrectPC (inr (p, g, b, e, a)).
+  Proof.
+    unfold isCorrectPC_range. move=> /(_ a) HH ?. apply HH. eauto.
+  Qed.
+
+  Lemma isCorrectPC_contiguous_range p g b e a0 an a l :
+    isCorrectPC_range p g b e a0 an →
+    contiguous_between l a0 an →
+    a ∈ l →
+    isCorrectPC (inr (p, g, b, e, a)).
+  Proof.
+    intros Hr Hc Hin.
+    eapply isCorrectPC_inrange; eauto.
+    eapply contiguous_between_middle_bounds'; eauto.
+  Qed.
+
+  Lemma isCorrectPC_range_perm p g b e a0 an :
+    isCorrectPC_range p g b e a0 an →
+    (a0 < an)%a →
+    p = RX ∨ p = RWX ∨ p = RWLX.
+  Proof.
+    intros Hr H0n.
+    assert (isCorrectPC (inr (p, g, b, e, a0))) as HH by (apply Hr; solve_addr).
+    inversion HH; auto.
+  Qed.
+
+  (* TODO: move to lang.v & simplify wp specs that require both isCorrectPC 
+     and withinBounds = true *)
+  Lemma isCorrectPC_withinBounds p g p' g' b e a :
+    isCorrectPC (inr (p, g, b, e, a)) →
+    withinBounds (p', g', b, e, a) = true.
+  Proof.
+    intros HH. inversion HH; subst.
+    rewrite /withinBounds !andb_true_iff Z.leb_le Z.ltb_lt. auto.
+  Qed.
 
   (* -------------------------------- LTACS ------------------------------------------- *)
   Ltac iPrologue_pre :=
@@ -46,10 +104,10 @@ Section stack_macros.
       let a' := fresh "a" in
       destruct a as [_ | a' a]; inversion Hlen; simpl
     end.
-  
+
   Ltac iPrologue prog :=
     (try iPrologue_pre);
-    iDestruct prog as "[Hi Hprog]"; 
+    iDestruct prog as "[Hi Hprog]";
     iApply (wp_bind (fill [SeqCtx])).
 
   Ltac iEpilogue prog :=
@@ -60,38 +118,30 @@ Section stack_macros.
     match goal with
     | Ha_first : ?a !! 0 = Some ?a_first |- _
     => apply Z.lt_trans with prev; auto; apply incr_list_lt_succ with a index; auto
-    end. 
-
-  Ltac iCorrectPC index :=
-    match goal with
-    | [ Hnext : contiguous ?a,
-          Ha_first : ?a !! 0 = Some ?a_first,
-          Ha_last : list.last ?a = Some ?a_last |- _ ]
-      => apply isCorrectPC_bounds_alt with a_first a_last; eauto; split ;
-         [ apply Z.lt_le_incl;auto |
-           apply incr_list_le_middle with a index; auto ]
     end.
 
-  Ltac addr_succ :=
-    match goal with
-    | H : _ |- (?a1 + ?z)%a = Some ?a2 =>
-      rewrite /incr_addr /=; do 2 f_equal; apply eq_proofs_unicity; decide equality
-    end.
+  Ltac iCorrectPC i j :=
+    eapply isCorrectPC_contiguous_range with (a0 := i) (an := j); eauto; [];
+    cbn; solve [ repeat constructor ].
+
+  Ltac iContiguous_next Ha index :=
+    apply contiguous_of_contiguous_between in Ha;
+    generalize (contiguous_spec _ Ha index); auto.
 
   (* --------------------------------------------------------------------------------- *)
   (* ------------------------- STACK MACROS AND THEIR SPECS -------------------------- *)
   (* --------------------------------------------------------------------------------- *)
-  
+
   (* -------------------------------------- PUSH ------------------------------------- *)
 
-  Definition push_r_instrs r_stk r := [lea_z r_stk 1 ; store_r r_stk r]. 
-                                
+  Definition push_r_instrs r_stk r := [lea_z r_stk 1 ; store_r r_stk r].
+
   Definition push_r (a1 a2 : Addr) (p : Perm) (r_stk r : RegName) : iProp Σ :=
-    ([∗ list] a;i ∈ [a1;a2];(push_r_instrs r_stk r), a ↦ₐ[p] i)%I. 
-  
+    ([∗ list] a;i ∈ [a1;a2];(push_r_instrs r_stk r), a ↦ₐ[p] i)%I.
+
   Lemma push_r_spec a1 a2 a3 w w' r p p' g b e stk_b stk_e stk_a stk_a' φ :
     isCorrectPC (inr ((p,g),b,e,a1)) ∧ isCorrectPC (inr ((p,g),b,e,a2)) →
-    PermFlows p p' -> 
+    PermFlows p p' ->
     withinBounds ((RWLX,Local),stk_b,stk_e,stk_a') = true →
     (a1 + 1)%a = Some a2 →
     (a2 + 1)%a = Some a3 →
@@ -107,12 +157,12 @@ Section stack_macros.
             -∗ WP Seq (Instr Executable) {{ φ }})
     ⊢
       WP Seq (Instr Executable) {{ φ }}.
-  Proof. 
+  Proof.
     iIntros ([Hvpc1 Hvpc2] Hfl Hwb Hsuc Hlea Hstk)
             "([Ha1 [Ha2 _] ] & HPC & Hr_stk & Hr & Hstk_a' & Hφ)".
     iApply (wp_bind (fill [SeqCtx])).
     iApply (wp_lea_success_z _ _ _ _ _ a1 a2 _ r_stk RWLX with "[HPC Ha1 Hr_stk]");
-      eauto; try apply lea_z_i; iFrame. 
+      eauto; try apply lea_z_i; iFrame.
     iNext. iIntros "(HPC & Ha1 & Hr_stk) /=".
     iApply wp_pure_step_later; auto. iNext.
     iApply (wp_bind (fill [SeqCtx])).
@@ -120,18 +170,18 @@ Section stack_macros.
               with "[HPC Ha2 Hr_stk Hr Hstk_a']"); eauto; try apply store_r_i;
       first apply PermFlows_refl; iFrame.
     iNext. iIntros "(HPC & Ha2 & Hr & Hr_stk & Hstk_a') /=".
-    iApply wp_pure_step_later; auto. iNext. iApply "Hφ". iFrame. done. 
+    iApply wp_pure_step_later; auto. iNext. iApply "Hφ". iFrame. done.
   Qed.
 
-  
-  Definition push_z_instrs r_stk z := [lea_z r_stk 1; store_z r_stk z]. 
-  
+
+  Definition push_z_instrs r_stk z := [lea_z r_stk 1; store_z r_stk z].
+
   Definition push_z (a1 a2 : Addr) (p : Perm) (r_stk : RegName) (z : Z) : iProp Σ :=
     ([∗ list] a;i ∈ [a1;a2];(push_z_instrs r_stk z), a ↦ₐ[p] i)%I.
-  
+
   Lemma push_z_spec a1 a2 a3 w z p p' g b e stk_b stk_e stk_a stk_a' φ :
     isCorrectPC (inr ((p,g),b,e,a1)) ∧ isCorrectPC (inr ((p,g),b,e,a2)) →
-    PermFlows p p' -> 
+    PermFlows p p' ->
     withinBounds ((RWLX,Local),stk_b,stk_e,stk_a') = true →
     (a1 + 1)%a = Some a2 →
     (a2 + 1)%a = Some a3 →
@@ -146,7 +196,7 @@ Section stack_macros.
             -∗ WP Seq (Instr Executable) {{ φ }})
     ⊢
       WP Seq (Instr Executable) {{ φ }}.
-  Proof. 
+  Proof.
     iIntros ([Hvpc1 Hvpc2] Hfl Hwb Hsuc Hlea Hstk)
             "([Ha1 [Ha2 _] ] & HPC & Hr_stk & Hstk_a' & Hφ)".
     iApply (wp_bind (fill [SeqCtx])).
@@ -159,20 +209,20 @@ Section stack_macros.
               with "[HPC Ha2 Hr_stk Hstk_a']"); eauto; first apply store_z_i;
       first apply PermFlows_refl; iFrame.
     iNext. iIntros "(HPC & Ha2 & Hr_stk & Hstk_a') /=".
-    iApply wp_pure_step_later; auto. iNext. iApply "Hφ". iFrame. done. 
+    iApply wp_pure_step_later; auto. iNext. iApply "Hφ". iFrame. done.
   Qed.
 
-  
+
   (* -------------------------------------- POP -------------------------------------- *)
   Definition pop_instrs r_stk r := [load_r r r_stk; sub_z_z r_t1 0 1; lea_r r_stk r_t1].
-  
+
   Definition pop (a1 a2 a3 : Addr) (p : Perm) (r_stk r : RegName) : iProp Σ :=
     ([∗ list] i;a ∈ (pop_instrs r_stk r);[a1;a2;a3], a ↦ₐ[p] i)%I.
 
   Lemma pop_spec a1 a2 a3 a4 r w w' wt1 p p' g b e stk_b stk_e stk_a stk_a' φ :
     isCorrectPC (inr ((p,g),b,e,a1)) ∧ isCorrectPC (inr ((p,g),b,e,a2)) ∧
     isCorrectPC (inr ((p,g),b,e,a3)) →
-    PermFlows p p' -> 
+    PermFlows p p' ->
     withinBounds ((RWLX,Local),stk_b,stk_e,stk_a) = true →
     r ≠ PC →
     (a1 + 1)%a = Some a2 →
@@ -203,98 +253,96 @@ Section stack_macros.
               with "[HPC Ha1 Hr_stk Hr Hstk_a]"); eauto; first apply load_r_i;
       first apply PermFlows_refl;iFrame.
     iNext. iIntros "(HPC & Hr & Ha1 & Hr_stk & Hstk_a) /=".
-    iApply wp_pure_step_later; auto; iNext. 
+    iApply wp_pure_step_later; auto; iNext.
     iApply (wp_bind (fill [SeqCtx])).
     iApply (wp_add_sub_lt_success _ r_t1 _ _ _ _ a2 with "[HPC Ha2 Hr_t1]");
       first (right;left;apply sub_z_z_i); eauto; iFrame; simpl.
     { iSplit; iPureIntro; reflexivity. }
     iNext.
-    rewrite sub_z_z_i Ha2'. 
+    rewrite sub_z_z_i Ha2'.
     iIntros "(HPC & Ha2 & _ & _ & Hr_t1) /=".
-    iApply wp_pure_step_later; auto; iNext. 
+    iApply wp_pure_step_later; auto; iNext.
     iApply (wp_bind (fill [SeqCtx])).
     iApply (wp_lea_success_reg _ _ _ _ _ a3 a4 _ r_stk _ RWLX
               with "[HPC Ha3 Hr_stk Hr_t1]"); eauto; first apply lea_r_i; iFrame.
     iNext. iIntros "(HPC & Ha3 & Hr_t1 & Hr_stk) /=".
     iApply wp_pure_step_later; auto; iNext.
-    iApply "Hφ". iFrame. done. 
+    iApply "Hφ". iFrame. done.
   Qed.
 
   (* -------------------------------------- RCLEAR ----------------------------------- *)
   (* the following macro clears registers in r. a denotes the list of addresses
      containing the instructions for the clear: |a| = |r| *)
-  Definition rclear_instrs (r : list RegName) := map (λ r_i, move_z r_i 0) r. 
-  
+  Definition rclear_instrs (r : list RegName) := map (λ r_i, move_z r_i 0) r.
+
   Definition rclear (a : list Addr) (p : Perm) (r : list RegName) : iProp Σ :=
       ([∗ list] k↦a_i;w_i ∈ a;(rclear_instrs r), a_i ↦ₐ[p] w_i)%I.
 
-  Lemma rclear_spec (a : list Addr) (r : list RegName) p p' g b e a1 an a' φ :
-    contiguous a →
-    list.last a = Some an → (an + 1)%a = Some a' →
+  Lemma rclear_spec (a : list Addr) (r : list RegName) p p' g b e a1 an φ :
+    contiguous_between a a1 an →
     ¬ PC ∈ r → hd_error a = Some a1 →
-    isCorrectPC (inr ((p,g),b,e,a1)) ∧ isCorrectPC (inr ((p,g),b,e,an)) →
+    isCorrectPC_range p g b e a1 an →
     PermFlows p p' →
-    
+
       ▷ (∃ ws, ([∗ list] k↦r_i;w_i ∈ r;ws, r_i ↦ᵣ w_i))
     ∗ ▷ PC ↦ᵣ inr ((p,g),b,e,a1)
-    ∗ ▷ rclear a p' r    
-    ∗ ▷ (PC ↦ᵣ inr ((p,g),b,e,a') ∗ ([∗ list] k↦r_i ∈ r, r_i ↦ᵣ inl 0%Z)
+    ∗ ▷ rclear a p' r
+    ∗ ▷ (PC ↦ᵣ inr ((p,g),b,e,an) ∗ ([∗ list] k↦r_i ∈ r, r_i ↦ᵣ inl 0%Z)
             ∗ rclear a p' r -∗
             WP Seq (Instr Executable) {{ φ }})
     ⊢ WP Seq (Instr Executable) {{ φ }}.
   Proof.
-    iIntros (Hsuc Hend Ha' Hne Hhd [Hvpchd Hvpcend] Hfl) "(>Hreg & >HPC & >Hrclear & Hφ)".
-    iDestruct (big_sepL2_length with "Hrclear") as %Har. 
-    iRevert (Hne Har Hhd Hvpchd). 
-    iInduction (a) as [_ | a1'] "IH" forall (r a1). iIntros (Hne Har Hhd Hvpchd).
-    inversion Hhd; simplify_eq.
-    iDestruct "Hreg" as (ws) "Hreg". 
-    iIntros (Hne Har Hhd Hvpchd).
+    iIntros (Ha Hne Hhd Hvpc Hfl) "(>Hreg & >HPC & >Hrclear & Hφ)".
+    iDestruct (big_sepL2_length with "Hrclear") as %Har.
+    iRevert (Hne Har Hhd Hvpc Ha).
+    iInduction (a) as [_ | a1'] "IH" forall (r a1 an). iIntros (Hne Har Hhd Hvpc Ha).
+    by inversion Hhd; simplify_eq.
+    iDestruct "Hreg" as (ws) "Hreg".
+    iIntros (Hne Har Hhd Hvpc Ha).
     iApply (wp_bind (fill [SeqCtx])). rewrite /rclear /=.
-    (* rewrite -(beq_nat_refl (length r)).  *)destruct r; inversion Har. 
+    (* rewrite -(beq_nat_refl (length r)).  *)destruct r; inversion Har.
     iDestruct (big_sepL2_cons with "Hrclear") as "[Ha1 Hrclear]".
     iDestruct (big_sepL2_length with "Hreg") as %rws.
-    destruct ws; inversion rws. 
+    destruct ws; inversion rws.
     iDestruct (big_sepL2_cons with "Hreg") as "[Hr Hreg]".
-    destruct a. 
-    - inversion H4; symmetry in H6; apply (nil_length_inv) in H6. 
-      inversion Hend. inversion Hhd. subst.                                      
+    destruct a.
+    - inversion H4; symmetry in H6; apply (nil_length_inv) in H6.
+      inversion Hhd. subst.
       iApply (wp_move_success_z _ _ _ _ _ a1 with "[HPC Ha1 Hr]");
-        eauto;first apply move_z_i.
+        eauto;first apply move_z_i; first iCorrectPC a1 an.
+      { eapply contiguous_between_last; eauto. }
       { apply (not_elem_of_cons) in Hne as [Hne _]. apply Hne. }
       iFrame. iNext. iIntros "(HPC & Han & Hr) /=".
-      iApply wp_pure_step_later; auto; iNext. 
-      iApply "Hφ". iFrame. destruct r0; inversion H6. done. 
-    - destruct r0; inversion H4.
+      iApply wp_pure_step_later; auto; iNext.
+      iApply "Hφ". iFrame. destruct r0; inversion H6. done.
+    - destruct r0; inversion H4. inversion Hhd; subst.
       iApply (wp_move_success_z _ _ _ _ _ a1 a _ r with "[HPC Ha1 Hr]")
-      ; eauto; first apply move_z_i. 
-      { apply Hsuc with 0; simpl; auto. }
+      ; eauto; first apply move_z_i; first iCorrectPC a1 an.
+      { iContiguous_next Ha 0. }
       { by apply not_elem_of_cons in Hne as [Hne _]. }
-      inversion Hhd. subst. 
       iFrame. iNext. iIntros "(HPC & Ha1 & Hr) /=".
       iApply wp_pure_step_later; auto. iNext.
-      inversion Hhd; subst.
-      iApply ("IH" with "[] [] [Hreg] [HPC] [Hrclear] [Hφ Ha1 Hr]"); iFrame. 
-      + iPureIntro. intros i ai aj Hai Haj.
-        apply Hsuc with (S i); simpl; eauto.
-      + auto.
-      + iExists (ws). iFrame. 
-        (* iApply big_sepL2_cons. iFrame.  *)
-      + simpl. rewrite H6. iFrame. 
-      + simpl. rewrite H6. 
+      rewrite -/(map _ _) -/(rclear_instrs _).
+      iApply ("IH" with "[Hreg] [HPC] [Hrclear] [Hφ Ha1 Hr]"); iFrame.
+      + iExists (ws). iFrame.
+      + simpl. rewrite H6. iFrame.
+      + simpl. rewrite H6.
         iNext. iIntros "(HPC & Hreg & Hrclear)".
-        iApply "Hφ". iFrame. 
-      + iPureIntro. by apply not_elem_of_cons in Hne as [_ Hne]. 
+        iApply "Hφ". iFrame.
+      + iPureIntro. by apply not_elem_of_cons in Hne as [_ Hne].
       + iPureIntro. simpl. congruence.
       + auto.
       + iPureIntro.
-        assert (a1 ≤ a)%Z as Hlow.
-        { apply Z.lt_le_incl. apply incr_list_lt_succ with (a1 :: a :: a0) 0; auto. }
-      assert (a ≤ an)%Z.
-      { apply incr_list_le_middle with (a1 :: a :: a0) 1; auto. }
-      apply isCorrectPC_bounds_alt with a1 an; auto. 
-  Qed. 
-  
+        intros a' [? Ha'].
+        assert (a1 <= a')%a as Hlow.
+        { enough (a1 <= a)%a by solve_addr.
+          eapply contiguous_between_middle_bounds'; eauto. repeat constructor. }
+        by specialize (Hvpc a' (conj Hlow Ha')).
+      + iPureIntro. inversion Ha; subst.
+        assert (a = a') as ->. eapply contiguous_between_cons_inv_first; eauto.
+        auto.
+  Qed.
+
   (* -------------------------------------- MCLEAR ----------------------------------- *)
    (* the following macro clears the region of memory a capability govers over. a denotes
      the list of adresses containing the instructions for the clear. |a| = 23 *)
@@ -302,9 +350,9 @@ Section stack_macros.
   (* first we will define the list of Words making up the mclear macro *)
   Definition mclear_instrs r_stk off_end off_iter :=
     [ move_r r_t4 r_stk;
-      getb r_t1 r_t4; 
-      geta r_t2 r_t4; 
-      sub_r_r r_t2 r_t1 r_t2; 
+      getb r_t1 r_t4;
+      geta r_t2 r_t4;
+      sub_r_r r_t2 r_t1 r_t2;
       lea_r r_t4 r_t2;
       gete r_t5 r_t4;
       sub_r_z r_t5 r_t5 1; (* we subtract the bound by one so that the lt check becomes a le check *)
@@ -314,11 +362,11 @@ Section stack_macros.
       lea_z r_t3 off_iter; (* offset to "iter" *)
     (* iter: *)
       lt_r_r r_t6 r_t5 r_t1;
-      store_z r_t4 0; 
       jnz r_t2 r_t6;
+      store_z r_t4 0;
       lea_z r_t4 1;
-      add_r_z r_t1 r_t1 1; 
-      jmp r_t3; 
+      add_r_z r_t1 r_t1 1;
+      jmp r_t3;
     (* end: *)
       move_z r_t4 0;
       move_z r_t1 0;
@@ -339,9 +387,19 @@ Section stack_macros.
   Proof.
     iIntros "Hr1 Hr2".
     iDestruct (mapsto_valid_2 with "Hr1 Hr2") as %?.
-    contradiction. 
-  Qed. 
-             
+    contradiction.
+  Qed.
+
+  Lemma region_size_S a b :
+    (a < b)%a ->
+    region_size a b = S (region_size (^(a+1))%a b).
+  Proof. rewrite /region_size. solve_addr. Qed.
+
+  Lemma region_size_0 a b :
+    (b <= a)%a ->
+    region_size a b = 0.
+  Proof. rewrite /region_size. solve_addr. Qed.
+
   Lemma mclear_iter_spec (a1 a2 a3 a4 a5 a6 b_r e_r a_r (* e_r' *) : Addr) ws (z : nat)
         p p' g b e rt rt1 rt2 rt3 rt4 rt5 a_end (p_r p_r' : Perm) (g_r : Locality) φ :
         isCorrectPC (inr ((p,g),b,e,a1))
@@ -355,13 +413,12 @@ Section stack_macros.
       ∧ (a3 + 1)%a = Some a4
       ∧ (a4 + 1)%a = Some a5
       ∧ (a5 + 1)%a = Some a6 →
-        withinBounds ((p_r,g_r),b_r,e_r,a_r) = true → (* This should now always hold! since we are jumping once a_r and e_r are equal *)
+        ((b_r + z < e_r)%Z → withinBounds ((p_r,g_r),b_r,e_r,a_r) = true) →
         writeAllowed p_r = true →
         (* (e_r + 1)%a = Some e_r' → *)
         (b_r + z)%a = Some a_r →
         PermFlows p p' ->
-        PermFlows p_r p_r' -> 
- 
+        PermFlows p_r p_r' ->
       ([[a_r,e_r]] ↦ₐ[p_r'] [[ws]]
      ∗ ▷ PC ↦ᵣ inr ((p,g),b,e,a1)
      ∗ ▷ rt ↦ᵣ inr ((p_r,g_r),b_r,e_r,a_r)
@@ -371,8 +428,8 @@ Section stack_macros.
      ∗ ▷ rt4 ↦ᵣ inr (p, g, b, e, a_end)
      ∗ ▷ rt5 ↦ᵣ inr (p, g, b, e, a1)
      ∗ ▷ ([∗ list] a_i;w_i ∈ [a1;a2;a3;a4;a5;a6];[lt_r_r rt3 rt2 rt1;
-                                                  store_z rt 0;
                                                   jnz rt4 rt3;
+                                                  store_z rt 0;
                                                   lea_z rt 1;
                                                   add_r_z rt1 rt1 1;
                                                   jmp rt5], a_i ↦ₐ[p'] w_i)
@@ -380,14 +437,14 @@ Section stack_macros.
              ∗ [[ a_r , e_r ]] ↦ₐ[p_r'] [[ region_addrs_zeroes a_r e_r ]]
              ∗ (∃ a_r, rt ↦ᵣ inr (p_r, g_r, b_r, e_r, a_r))
              ∗ rt5 ↦ᵣ inr (p, g, b, e, a1)
-             ∗ a2 ↦ₐ[p'] store_z rt 0
+             ∗ a3 ↦ₐ[p'] store_z rt 0
              ∗ a4 ↦ₐ[p'] lea_z rt 1
              ∗ a5 ↦ₐ[p'] add_r_z rt1 rt1 1
              ∗ a6 ↦ₐ[p'] jmp rt5
              ∗ a1 ↦ₐ[p'] lt_r_r rt3 rt2 rt1
              ∗ rt2 ↦ᵣ inl ((z_of e_r) - 1)%Z
              ∗ (∃ z, rt1 ↦ᵣ inl (b_r + z)%Z)
-             ∗ a3 ↦ₐ[p'] jnz rt4 rt3
+             ∗ a2 ↦ₐ[p'] jnz rt4 rt3
              ∗ rt4 ↦ᵣ inr (p, g, b, e, a_end)
              ∗ rt3 ↦ᵣ inl 1%Z
               -∗ WP Seq (Instr Executable) {{ φ }})
@@ -395,10 +452,10 @@ Section stack_macros.
   Proof.
     iIntros (Hvpc Hnext Hwb Hwa (* Her' *) Hprogress Hfl1 Hfl2)
             "(Hbe & >HPC & >Hrt & >Hr_t1 & >Hr_t2 & >Hr_t3 & >Hr_t4 & >Hr_t5 & >Hprog & Hφ)".
-    iRevert (Hwb Hprogress). 
+    iRevert (Hwb Hprogress).
     iLöb as "IH" forall (a_r ws z).
     iIntros (Hwb Hprogress).
-    iDestruct "Hr_t3" as (w) "Hr_t3". 
+    iDestruct "Hr_t3" as (w) "Hr_t3".
     destruct Hvpc as (Hvpc1 & Hvpc2 & Hvpc3 & Hvpc4 & Hvpc5 & Hvpc6).
     destruct Hnext as (Hnext1 & Hnext2 & Hnext3 & Hnext4 & Hnext5).
     iAssert (⌜rt1 ≠ PC⌝)%I as %Hne1.
@@ -417,182 +474,113 @@ Section stack_macros.
     { destruct (reg_eq_dec rt1 rt3); auto. rewrite e0.
         by iDestruct (regname_dupl_false with "Hr_t1 Hr_t3") as "Hfalse". }
     (* lt rt3 rt2 rt1 *)
-    iDestruct "Hprog" as "[Hi Hprog]". 
+    iDestruct "Hprog" as "[Hi Hprog]".
     iApply (wp_bind (fill [SeqCtx])).
     iApply (wp_add_sub_lt_success _ rt3 _ _ _ _ a1 _ _ (inr rt2) (inr rt1) _ _
               with "[Hi HPC Hr_t3 Hr_t1 Hr_t2]"); first (right;right;apply lt_i);
-      first apply Hfl1; eauto. 
+      first apply Hfl1; eauto.
     destruct (reg_eq_dec rt2 rt3),(reg_eq_dec rt1 rt3),(reg_eq_dec rt3 PC);iFrame.
     destruct (reg_eq_dec rt3 PC); try contradiction.
-    rewrite Hnext1 lt_i. 
+    rewrite Hnext1 lt_i.
     iEpilogue "(HPC & Ha1 & Hr_t2 & Hr_t1 & Hr_t3)".
-    destruct (reg_eq_dec rt2 rt3),(reg_eq_dec rt1 rt3); try contradiction. 
-    rewrite /region_mapsto /region_addrs. 
-    destruct (Z_le_dec (b_r + z) (e_r - 1))%Z; simpl. 
+    destruct (reg_eq_dec rt2 rt3),(reg_eq_dec rt1 rt3); try contradiction.
+    rewrite /region_mapsto /region_addrs.
+    destruct (Z_le_dec (b_r + z) (e_r - 1))%Z; simpl.
     - assert (Z.b2z (e_r - 1 <? b_r + z)%Z = 0%Z) as Heq0.
-      { rewrite /Z.b2z. assert (e_r - 1 <? b_r + z = false)%Z as Heq; [apply Z.ltb_nlt; omega|].
-          by rewrite Heq. }
-      rewrite Heq0. 
+      { rewrite /Z.b2z. destruct (e_r - 1 <? b_r + z)%Z eqn:HH; auto.
+        apply Z.ltb_lt in HH. lia. }
+      rewrite Heq0.
+      (* jnz rt4 rt3 *)
+      iDestruct "Hprog" as "[Hi Hprog]".
+      iApply (wp_bind (fill [SeqCtx])).
+      iApply (wp_jnz_success_next _ rt4 rt3 _ _ _ _ a2 a3 with "[HPC Hi Hr_t3]");
+        first apply jnz_i; first apply Hfl1;eauto.
+      iFrame. iEpilogue "(HPC & Ha2 & Hr_t3)".
       (* store rt 0 *)
       rewrite/ withinBounds in Hwb.
-      apply andb_prop in Hwb as [Hwb_b Hwb_e]. 
-      apply (Z.leb_le a_r e_r) in Hwb_e. 
-      destruct (Z_le_dec a_r e_r); try contradiction.
-      destruct ws as [_ | w1 ws]; [simpl; by iApply bi.False_elim|simpl]. 
+      apply andb_prop in Hwb as [Hwb_b%Z.leb_le Hwb_e%Z.ltb_lt].
+      rewrite {1}region_size_S /=.
+      destruct ws as [| w1 ws]; simpl; [by iApply bi.False_elim|].
       iDestruct "Hbe" as "[Ha_r Hbe]".
-      iDestruct "Hprog" as "[Hi Hprog]". 
-      iApply (wp_bind (fill [SeqCtx])). 
-      iApply (wp_store_success_z _ _ _ _ _ a2 a3 _ rt 0 _ p_r g_r b_r e_r a_r with "[HPC Hi Hrt Ha_r]"); first apply store_z_i; first apply Hfl1; eauto.
-      { split;[auto|]. rewrite /withinBounds andb_true_iff; split;[auto|]. by apply Z.leb_le. }
-      iFrame. iEpilogue "(HPC & Ha2 & Hrt & Ha_r)".
-      (* jnz rt4 rt3 *)
-      iDestruct "Hprog" as "[Hi Hprog]". 
-      iApply (wp_bind (fill [SeqCtx])). 
-      iApply (wp_jnz_success_next _ rt4 rt3 _ _ _ _ a3 a4 with "[HPC Hi Hr_t3]");
-        first apply jnz_i; first apply Hfl1;eauto. 
-      iFrame. iEpilogue "(HPC & Ha3 & Hr_t3)". 
+      iDestruct "Hprog" as "[Hi Hprog]".
+      iApply (wp_bind (fill [SeqCtx])).
+      iApply (wp_store_success_z _ _ _ _ _ a3 a4 _ rt 0 _ p_r g_r b_r e_r a_r with "[HPC Hi Hrt Ha_r]"); first apply store_z_i; first apply Hfl1; eauto.
+      { split;[auto|]. rewrite /withinBounds andb_true_iff; split;[auto|].
+          by apply Z.leb_le. by apply Z.ltb_lt. }
+      iFrame. iEpilogue "(HPC & Ha3 & Hrt & Ha_r)".
       (* lea rt 1 *)
       assert (∃ a_r', (a_r + 1)%a = Some a_r') as [a_r' Ha_r'].
       { apply addr_next_lt with e_r. apply incr_addr_of_z_i in Hprogress. lia. }
-      iDestruct "Hprog" as "[Hi Hprog]". 
-      iApply (wp_bind (fill [SeqCtx])). 
-      iApply (wp_lea_success_z _ _ _ _ _ a4 a5 _ rt p_r _ _ _ a_r 1 a_r' with "[HPC Hi Hrt]"); first apply lea_z_i; first apply Hfl1; eauto. 
+      iDestruct "Hprog" as "[Hi Hprog]".
+      iApply (wp_bind (fill [SeqCtx])).
+      iApply (wp_lea_success_z _ _ _ _ _ a4 a5 _ rt p_r _ _ _ a_r 1 a_r' with "[HPC Hi Hrt]"); first apply lea_z_i; first apply Hfl1; eauto.
       { destruct p_r; auto. }
       iFrame. iEpilogue "(HPC & Ha4 & Hrt)".
       (* add rt1 rt1 1 *)
-      iDestruct "Hprog" as "[Hi Hprog]". 
-      iApply (wp_bind (fill [SeqCtx])). 
+      iDestruct "Hprog" as "[Hi Hprog]".
+      iApply (wp_bind (fill [SeqCtx])).
       iApply (wp_add_sub_lt_success _ rt1 _ _ _ _ a5 _ _ (inr rt1) with "[HPC Hi Hr_t1]");
-        first (left;apply add_r_z_i); first apply Hfl1; eauto. 
+        first (left;apply add_r_z_i); first apply Hfl1; eauto.
       { iFrame. iSplit; eauto. by destruct (reg_eq_dec rt1 rt1); try contradiction. }
       destruct (reg_eq_dec rt1 PC),(reg_eq_dec rt1 rt1); try contradiction.
-      rewrite Hnext5 add_r_z_i. 
+      rewrite Hnext5 add_r_z_i.
       iEpilogue "(HPC & Ha5 & _ & _ & Hr_t1)".
       (* jmp rt5 *)
-      iDestruct "Hprog" as "[Hi _]". 
-      iApply (wp_bind (fill [SeqCtx])). 
+      iDestruct "Hprog" as "[Hi _]".
+      iApply (wp_bind (fill [SeqCtx])).
       iApply (wp_jmp_success _ _ _ _ _ a6 with "[HPC Hi Hr_t5]");
-        first apply jmp_i; first apply Hfl1; eauto. 
+        first apply jmp_i; first apply Hfl1; eauto.
       iFrame. iEpilogue "(HPC & Ha6 & Hr_t5)".
       iApply ("IH" $! a_r' ws (z + 1)%nat with
                   "[Hbe] [HPC] [Hrt] [Hr_t1] [Hr_t2] [Hr_t3] [Hr_t4] [Hr_t5] [Ha1 Ha2 Ha3 Ha4 Ha5 Ha6] [Hφ Ha_r]")
-      ; iFrame. 
-      + rewrite Ha_r'; simpl.
-        destruct (Z_le_dec a_r' e_r) as [Hle | Hle].
-        { assert (∀ {A : Type} (x : A) (l : list A), x :: l = [x] ++ l) as Hl; auto.
-          assert ((a_r < e_r)%Z).
-          { apply Z.lt_le_trans with a_r'; eauto.
-            rewrite /incr_addr in Ha_r'.
-            destruct (Z_le_dec (a_r + 1)%Z MemNum); inversion Ha_r'. simpl. omega.
-          }
-          rewrite Hl region_addrs_aux_singleton (region_addrs_aux_decomposition _ _ 1); last lia. 
-          destruct ws; simpl; first by iApply bi.False_elim.
-          iDestruct "Hbe" as "[$ Hbe]".
-          rewrite (addr_abs_next _ _ a_r'); auto. 
-        }
-        { apply Znot_le_gt in Hle.
-          apply Zle_lt_or_eq in Hwb_e as [Hlt | ->]. 
-          - apply (addr_next_lt_gt_contr a_r e_r a_r') in Hlt; auto; lia.
-          - rewrite Z.sub_diag. iFrame.
-        }
+      ; iFrame. all: auto.
+      + by rewrite Ha_r'.
       + assert (updatePcPerm (inr (p, g, b, e, a1)) = (inr (p, g, b, e, a1))).
         { rewrite /updatePcPerm. destruct p; auto.
           inversion Hvpc1; destruct H9 as [Hc | [Hc | Hc] ]; inversion Hc. }
         rewrite H3. iFrame.
       + assert (b_r + z + 1 = b_r + (z + 1)%nat)%Z as ->;[lia|]. iFrame.
-      + iExists (inl 0%Z). iFrame.
       + iNext.
         iIntros "(HPC & Hregion & Hrt & Hrt5 & Ha3 & Ha4 & Ha5 & Ha6 & Ha1 & Hrt2 & Hrt1 & Ha2 & Hrt4 & Hrt3)".
         iApply "Hφ".
         iFrame.
         rewrite /region_addrs_zeroes.
-        destruct (Z_le_dec a_r' e_r) as [Hle | Hle].
-        { destruct (Z_le_dec a_r e_r); last by iApply bi.False_elim.
-          simpl. iFrame.
-          assert ((z_of a_r) + 1 = z_of a_r')%Z.
-          { rewrite /incr_addr in Ha_r'.
-              by destruct (Z_le_dec (a_r + 1)%Z MemNum); inversion Ha_r'. }
-          assert ((e_r - a_r) = (Z.succ (e_r - a_r')))%Z; first lia. 
-          rewrite H4 Ha_r' /=.
-          rewrite Zabs2Nat.inj_succ; last lia.
-          rewrite /=. iFrame. }
-        { apply Znot_le_gt in Hle.
-          apply Zle_lt_or_eq in Hwb_e as [Hlt | Heq]. 
-          - apply (addr_next_lt_gt_contr a_r e_r a_r') in Hlt; auto; lia.
-          - rewrite Heq.
-            apply z_of_eq in Heq. 
-            rewrite Heq. 
-            rewrite /region_size Z.sub_diag. simpl.
-            destruct (Z_le_dec e_r e_r); last lia. 
-            simpl. iFrame. } 
-      + iPureIntro.
-        apply andb_true_intro.
-        apply Z.leb_le in Hwb_b. 
-        split; apply Z.leb_le.
-        * apply Z.le_trans with a_r; auto.
-          rewrite /incr_addr in Ha_r'.
-          destruct (Z_le_dec (a_r + 1)%Z MemNum); inversion Ha_r'; simpl; omega.  
-        * assert ((z_of b_r) + z = z_of a_r)%Z as Heq_brz.
-          { rewrite /incr_addr in Hprogress.
-              by destruct (Z_le_dec (b_r + z)%Z MemNum); inversion Hprogress. }
-          assert ((z_of a_r) + 1 = z_of a_r')%Z as Ha_rz.
-          { rewrite /incr_addr in Ha_r'.
-              by destruct (Z_le_dec (a_r + 1)%Z MemNum); inversion Ha_r'. }
-          lia. 
-      + iPureIntro.
-        rewrite -Ha_r'.
-        rewrite PeanoNat.Nat.add_1_r Nat2Z.inj_succ -Z.add_1_r. 
-        by rewrite (addr_add_assoc _ a_r). 
-    - assert (Z.b2z (e_r -1 <? b_r + z)%Z = 1%Z) as Heq0.
-      { rewrite /Z.b2z. assert (e_r - 1 <? b_r + z = true)%Z as Heq; [apply Z.ltb_lt; omega|].
-          by rewrite Heq. }
+        rewrite (region_size_S a_r e_r) //= (_: (^(a_r+1))%a = a_r'); [| solve_addr].
+        iFrame.
+      + iPureIntro. intro.
+        rewrite andb_true_iff -Zle_is_le_bool -Zlt_is_lt_bool. solve_addr.
+      + iPureIntro. solve_addr.
+      + solve_addr.
+    - assert (Z.b2z (e_r - 1 <? b_r + z)%Z = 1%Z) as Heq0.
+      { rewrite /Z.b2z. destruct (e_r - 1 <? b_r + z)%Z eqn:HH; auto.
+        apply Z.ltb_nlt in HH. lia. }
       rewrite Heq0.
-      assert (a_r >= e_r)%Z.
-      { assert ((z_of b_r) + z = a_r)%Z; 
-          first (rewrite /incr_addr in Hprogress;
-                   by destruct (Z_le_dec (b_r + z)%Z MemNum); inversion Hprogress).
-        rewrite -H3. lia. 
-      }
-      destruct (Z_le_dec a_r e_r).
-      + assert (z_of a_r = z_of e_r) as Heq;[lia|].
-        apply z_of_eq in Heq. subst. rewrite Z.sub_diag /=.
-        destruct ws;[by iApply bi.False_elim|]. 
-        iSimpl in "Hbe". iDestruct "Hbe" as "[He_r _]".
-        iDestruct "Hprog" as "[Hi Hprog]". 
-        iApply (wp_bind (fill [SeqCtx])). 
-        iApply (wp_store_success_z _ _ _ _ _ a2 a3 _ rt 0 _ p_r g_r b_r e_r e_r with "[HPC Hi Hrt He_r]"); first apply store_z_i; first apply Hfl1; eauto.
-        iFrame. iEpilogue "(HPC & Ha2 & Hrt & Ha_r)".
-        (* jnz *)
-        iDestruct "Hprog" as "[Hi Hprog]". 
-        iApply (wp_bind (fill [SeqCtx])). 
-        iApply (wp_jnz_success_jmp _ rt4 rt3 _ _ _ _ a3 _ _ (inl 1%Z) with "[HPC Hi Hr_t3 Hr_t4]"); first apply jnz_i; first apply Hfl1; eauto. 
-        iFrame. iEpilogue "(HPC & Ha3 & Hr_t4 & Hr_t3)". 
-        iApply "Hφ". iDestruct "Hprog" as "(Ha4 & Ha5 & Ha6 & _)". iFrame. 
-        rewrite /region_addrs_zeroes /= Z.sub_diag /=.
-        destruct (Z_le_dec e_r e_r);[|contradiction]. 
-        iFrame. iSplitR;[auto|].
-        iSplitL "Hrt". iExists (e_r). iFrame. iExists z. iFrame.
-      + (* This should lead to a contradiction from within bounds *)
-        exfalso. 
-        rewrite /withinBounds in Hwb.
-        apply andb_true_iff in Hwb as [Hwb1 Hwb2].
-        apply Z.leb_le in Hwb2. done. 
-        Unshelve. apply w1. 
-  Qed. 
+      assert (e_r <= a_r)%Z by solve_addr.
+      (* destruct (Z_le_dec a_r e_r). *)
+      rewrite region_size_0 //=.
+      destruct ws;[|by iApply bi.False_elim].
+      (* jnz *)
+      iDestruct "Hprog" as "[Hi Hprog]".
+      iApply (wp_bind (fill [SeqCtx])).
+      iApply (wp_jnz_success_jmp _ rt4 rt3 _ _ _ _ a2 _ _ (inl 1%Z) with "[HPC Hi Hr_t3 Hr_t4]"); first apply jnz_i; first apply Hfl1; eauto.
+      iFrame. iEpilogue "(HPC & Ha2 & Hr_t4 & Hr_t3)".
+      iApply "Hφ". iDestruct "Hprog" as "(Ha3 & Ha4 & Ha5 & Ha6 & _)".
+      rewrite /region_addrs_zeroes region_size_0 //=. iFrame.
+      iSplitL "Hrt"; eauto.
+      Unshelve. apply w1.
+  Qed.
 
-    
-  Lemma mclear_spec (a : list Addr) (r : RegName) 
-        (a_last a_first a6' a_end : Addr) p p' g b e p_r p_r' g_r (b_r e_r a_r : Addr) a' φ :
-    contiguous a →
-    a !! 0 = Some a_first → list.last a = Some a_last →
+
+  Lemma mclear_spec (a : list Addr) (r : RegName)
+        (a_first a6' a_end : Addr) p p' g b e p_r p_r' g_r (b_r e_r a_r : Addr) a' φ :
+    contiguous_between a a_first a' →
     (* We will assume that we are not trying to clear memory in a *)
     r ≠ PC ∧ writeAllowed p_r = true →
     (a !! 7 = Some a6' ∧ (a6' + 10)%a = Some a_end ∧ a !! 17 = Some a_end) →
-    
-    isCorrectPC (inr ((p,g),b,e,a_first)) → isCorrectPC (inr ((p,g),b,e,a_last)) →
-    PermFlows p p' → PermFlows p_r p_r' -> 
-    
-    (a_last + 1)%a = Some a' →
+
+    isCorrectPC_range p g b e a_first a' →
+    PermFlows p p' → PermFlows p_r p_r' ->
+
     (* We will also assume the region to clear is non empty *)
     (b_r ≤ e_r)%Z →
 
@@ -615,11 +603,11 @@ Section stack_macros.
             ∗ r_t6 ↦ᵣ inl 0%Z
             ∗ r ↦ᵣ inr ((p_r,g_r),b_r,e_r,a_r)
             ∗ [[ b_r , e_r ]] ↦ₐ[p_r'] [[region_addrs_zeroes b_r e_r]]
-            ∗ mclear a p' r 10 2 -∗ 
+            ∗ mclear a p' r 10 2 -∗
             WP Seq (Instr Executable) {{ φ }})
-    ⊢ WP Seq (Instr Executable) {{ φ }})%I.  
+    ⊢ WP Seq (Instr Executable) {{ φ }})%I.
   Proof.
-    iIntros (Hnext Ha_first Ha_last [Hne Hwa] Hjnz_off Hvpc1 Hvpc2 Hfl1 Hfl2 Ha_last' Hle)
+    iIntros (Hnext [Hne Hwa] Hjnz_off Hvpc Hfl1 Hfl2 Hle)
             "(Hmclear & >HPC & >Hr & >Hr_t4 & >Hr_t1 & >Hr_t2 & >Hr_t3 & >Hr_t5 & >Hr_t6 & >Hregion & Hφ)".
     iDestruct "Hr_t4" as (w4) "Hr_t4".
     iDestruct "Hr_t1" as (w1) "Hr_t1".
@@ -632,70 +620,61 @@ Section stack_macros.
     { destruct (((length a) =? (length (mclear_instrs r _ _)))%nat) eqn:Hlen; auto.
       rewrite /mclear Hlen. by iApply bi.False_elim. }
     rewrite /mclear Hlen /mclear_instrs; simpl in Hlen. apply beq_nat_true in Hlen.
-    destruct a as [_ | a1 a]; inversion Hlen; simpl; inversion Ha_first; simplify_eq. 
-    iPrologue "Hmclear". 
+    destruct a as [_ | a1 a]; inversion Hlen; simpl.
+    move: (contiguous_between_cons_inv_first _ _ _ _ Hnext).
+    match goal with |- (?a = _) -> _ => intro; subst a end.
+    iPrologue "Hmclear".
     iApply (wp_move_success_reg _ _ _ _ _ a_first _ _ r_t4 _ r with "[HPC Hr Hr_t4 Hi]");
-      first apply move_r_i; first apply Hfl1; eauto. 
-    iFrame. iEpilogue "(HPC & Ha_first & Hr_t4 & Hr)". 
+      first apply move_r_i; first apply Hfl1; first iCorrectPC a_first a'; eauto.
+    { iContiguous_next Hnext 0. }
+    iFrame. iEpilogue "(HPC & Ha_first & Hr_t4 & Hr)".
     (* getb r_t1 r_t4 *)
-    iPrologue "Hprog". 
-    assert (a_first < a0)%Z as Hlt0; first (apply incr_list_lt_succ with (a_first :: a0 :: a1 :: a) 0; auto). 
+    iPrologue "Hprog".
     iApply (wp_GetB_success _ r_t1 r_t4 _ _ _ _ a0 _ _ _ a1 with "[HPC Hi Hr_t1 Hr_t4]");
-      first apply getb_i; first apply Hfl1; first iCorrectPC 1; eauto. 
-    { apply Hnext with 1; auto. }
+      first apply getb_i; first apply Hfl1; first iCorrectPC a_first a'; eauto.
+    { iContiguous_next Hnext 1. }
     iFrame. iEpilogue "(HPC & Ha0 & Hr_t4 & Hr_t1)".
-    destruct (reg_eq_dec PC r_t4) as [Hcontr | _]; [inversion Hcontr|]. 
-    iCombine "Ha0 Ha_first" as "Hprog_done". 
+    destruct (reg_eq_dec PC r_t4) as [Hcontr | _]; [inversion Hcontr|].
+    iCombine "Ha0 Ha_first" as "Hprog_done".
     (* geta r_t2 r_t4 *)
-    iPrologue "Hprog". 
-    assert (a_first < a1)%Z as Hlt1; first middle_lt a0 1. 
+    iPrologue "Hprog".
     iApply (wp_GetA_success _ r_t2 r_t4 _ _ _ _ a1 _ _ _ a2 with "[HPC Hi Hr_t2 Hr_t4]");
-       first apply geta_i; first apply Hfl1; first iCorrectPC 2; auto. 
-    { apply Hnext with 2; auto. }
+       first apply geta_i; first apply Hfl1; first iCorrectPC a_first a'; auto.
+    { iContiguous_next Hnext 2. }
     iFrame. iEpilogue "(HPC & Ha1 & Hr_t4 & Hr_t2)".
-    destruct (reg_eq_dec PC r_t4) as [Hcontr | _]; [inversion Hcontr|]. 
-    iCombine "Ha1 Hprog_done" as "Hprog_done". 
+    destruct (reg_eq_dec PC r_t4) as [Hcontr | _]; [inversion Hcontr|].
+    iCombine "Ha1 Hprog_done" as "Hprog_done".
     (* sub r_t2 r_t1 r_t2 *)
     iPrologue "Hprog".
-    assert (a_first < a2)%Z as Hlt2; first middle_lt a1 2.
-    destruct b_r eqn:Hb_r. 
+    destruct b_r eqn:Hb_r.
     iApply (wp_add_sub_lt_success _ r_t2 _ _ _ _ a2 _ _ (inr r_t1) (inr r_t2)
-              with "[HPC Hi Hr_t1 Hr_t2]"); 
-      first (right; left; apply sub_r_r_i); first apply Hfl1; first iCorrectPC 3; eauto. 
+              with "[HPC Hi Hr_t1 Hr_t2]");
+      first (right; left; apply sub_r_r_i); first apply Hfl1; first iCorrectPC a_first a'; eauto.
     iFrame.
     destruct (reg_eq_dec PC r_t4) as [Hcontr | _]; [inversion Hcontr|].
     destruct (reg_eq_dec r_t2 PC) as [Hcontr | _]; [inversion Hcontr|].
     destruct (reg_eq_dec r_t1 r_t2) as [Hcontr | _]; [inversion Hcontr|].
     destruct (reg_eq_dec r_t2 r_t2); try contradiction.
     assert ((a2 + 1) = Some a3)%a as ->.
-    { apply Hnext with 3; auto. }
-    rewrite sub_r_r_i. 
+    { iContiguous_next Hnext 3. }
+    rewrite sub_r_r_i.
     iEpilogue "(HPC & Ha2 & Hr_t1 & _ & Hr_t2)".
-    iCombine "Ha2 Hprog_done" as "Hprog_done". 
+    iCombine "Ha2 Hprog_done" as "Hprog_done".
     (* lea r_t4 r_t2 *)
     iPrologue "Hprog".
-    assert (a_first < a3)%Z as Hlt3; first middle_lt a2 3.
     assert (a_r + (b_r - a_r) = b_r)%Z as Haddmin; first lia.
-    assert ((a_r + (b_r - a_r))%a = Some b_r) as Ha_rb_r.
-    { rewrite /incr_addr.
-      destruct (Z_le_dec (a_r + (b_r - a_r))%Z MemNum).
-      - f_equal. destruct b_r. apply addr_unique. done.
-      - exfalso. destruct b_r. rewrite Haddmin /= in n.
-        destruct Haddmin. 
-        apply Z.leb_nle in n. congruence. 
-    }
+    assert ((a_r + (b_r - a_r))%a = Some b_r) as Ha_rb_r by solve_addr.
     iApply (wp_lea_success_reg _ _ _ _ _ a3 a4 _ r_t4 r_t2 p_r _ _ _ a_r (b_r - a_r) with "[HPC Hi Hr_t4 Hr_t2]");
-      first apply lea_r_i; first apply Hfl1; first iCorrectPC 4; eauto.
-    { apply Hnext with 4; auto. }
+      first apply lea_r_i; first apply Hfl1; first iCorrectPC a_first a'; eauto.
+    { iContiguous_next Hnext 4. }
     { destruct p_r; inversion Hwa; auto. }
     rewrite /z_of Hb_r; iFrame. iEpilogue "(HPC & Ha3 & Hr_t2 & Hr_t4)".
-    iCombine "Ha3 Hprog_done" as "Hprog_done". 
+    iCombine "Ha3 Hprog_done" as "Hprog_done".
     (* gete r_t2 r_t4 *)
     iPrologue "Hprog".
-    assert (a_first < a4)%Z as Hlt4; first middle_lt a3 4.
     iApply (wp_GetE_success _ r_t5 _ _ _ _ _ a4 _ _ _ a5 with "[HPC Hi Hr_t5 Hr_t4]");
-      first apply gete_i; first apply Hfl1; first iCorrectPC 5; eauto. 
-    { apply Hnext with 5; auto. }
+      first apply gete_i; first apply Hfl1; first iCorrectPC a_first a'; eauto.
+    { iContiguous_next Hnext 5. }
     do 2 iFrame.
     destruct (reg_eq_dec PC r_t4) as [Hcontr | _]; [inversion Hcontr|].
     destruct (reg_eq_dec r_t4 r_t5) as [Hcontr | _]; [inversion Hcontr|].
@@ -703,55 +682,54 @@ Section stack_macros.
     iCombine "Ha4 Hprog_done" as "Hprog_done".
     (* sub r_t5 r_t5 1 *)
     iPrologue "Hprog".
-    assert (a_first < a5)%Z as Hlt5; first middle_lt a4 5.
     iApply (wp_add_sub_lt_success with "[$HPC $Hi Hr_t5]");
-      [right;left;apply sub_r_z_i|apply Hfl1|iCorrectPC 6|auto..].
+      [right;left;apply sub_r_z_i|apply Hfl1|iCorrectPC a_first a'|auto..].
     destruct (reg_eq_dec r_t5 PC) eqn:Hcontr;[by inversion Hcontr|clear Hcontr].
-    assert ((a5 + 1)%a = Some a6) as ->;[apply Hnext with 6; auto|].
+    assert ((a5 + 1)%a = Some a6) as ->.
+    { iContiguous_next Hnext 6. }
     destruct (reg_eq_dec r_t5 r_t5) eqn:Hcontr;[clear Hcontr|by inversion Hcontr].
     rewrite sub_r_z_i.
     iEpilogue "(HPC & Ha5 & _ & _ & Hr_t5)".
-    iCombine "Ha5 Hprog_done" as "Hprog_done". 
+    iCombine "Ha5 Hprog_done" as "Hprog_done".
     (* move r_t2 PC *)
     iPrologue "Hprog".
-    assert (a_first < a6)%Z as Hlt6; first middle_lt a5 6.
     iApply (wp_move_success_reg_fromPC _ _ _ _ _ a6 a7 _ r_t2 with "[HPC Hi Hr_t2]");
-      first apply move_r_i; first apply Hfl1; first iCorrectPC 7; eauto. 
-    { apply Hnext with 7; auto. }
+      first apply move_r_i; first apply Hfl1; first iCorrectPC a_first a'; eauto.
+    { iContiguous_next Hnext 7. }
     iFrame. iEpilogue "(HPC & Ha6 & Hr_t2)".
-    iCombine "Ha6 Hprog_done" as "Hprog_done". 
+    iCombine "Ha6 Hprog_done" as "Hprog_done".
     (* lea r_t2 off_end *)
     iPrologue "Hprog".
-    assert (a_first < a7)%Z as Hlt7; first middle_lt a6 7.
     assert (p ≠ E) as Hpne.
-    { inversion Hvpc1; destruct H19 as [? | [? | ?] ]; subst; auto. }
+    { have: (isCorrectPC (inr (p, g, b, e, a_first))).
+      { apply Hvpc. eapply contiguous_between_middle_bounds'; eauto. constructor. }
+      inversion 1; subst.
+      destruct H19 as [? | [? | ?] ]; subst; auto. }
     iApply (wp_lea_success_z _ _ _ _ _ a7 a8 _ r_t2 p _ _ _ a6 10 a_end with "[HPC Hi Hr_t2]");
-      first apply lea_z_i; first apply Hfl1; first iCorrectPC 8; auto.
-    { apply Hnext with 8; auto. }
+      first apply lea_z_i; first apply Hfl1; first iCorrectPC a_first a'; auto.
+    { iContiguous_next Hnext 8. }
     { destruct Hjnz_off as (Ha7' & Hoff_end & Ha_end). simpl in Ha7'. congruence. }
     iFrame. iEpilogue "(HPC & Ha7 & Hr_t2)".
-    iCombine "Ha7 Hprog_done" as "Hprog_done". 
+    iCombine "Ha7 Hprog_done" as "Hprog_done".
     (* move r_t3 PC *)
     iPrologue "Hprog".
-    assert (a_first < a8)%Z as Hlt8; first middle_lt a7 8.
     iApply (wp_move_success_reg_fromPC _ _ _ _ _ a8 a9 _ r_t3 with "[HPC Hi Hr_t3]");
-      first apply move_r_i; first apply Hfl1; first iCorrectPC 9; auto.
-    { apply Hnext with 9; auto. }
+      first apply move_r_i; first apply Hfl1; first iCorrectPC a_first a'; auto.
+    { iContiguous_next Hnext 9. }
     iFrame. iEpilogue "(HPC & Ha8 & Hr_t3)".
-    iCombine "Ha8 Hprog_done" as "Hprog_done". 
+    iCombine "Ha8 Hprog_done" as "Hprog_done".
     (* lea r_t3 off_iter *)
     iPrologue "Hprog".
-    assert (a_first < a9)%Z as Hlt9; first middle_lt a8 9.
     iApply (wp_lea_success_z _ _ _ _ _ a9 a10 _ r_t3 p _ _ _ a8 2 a10 with "[HPC Hi Hr_t3]");
-      first apply lea_z_i; first apply Hfl1; first iCorrectPC 10; auto.
-    { apply Hnext with 10; auto. }
-    { assert (2 = 1 + 1)%Z as ->; auto. 
-      apply incr_addr_trans with a9. 
-      apply Hnext with 9; auto. apply Hnext with 10; auto. }
+      first apply lea_z_i; first apply Hfl1; first iCorrectPC a_first a'; auto.
+    { iContiguous_next Hnext 10. }
+    { assert (2 = 1 + 1)%Z as ->; auto.
+      apply incr_addr_trans with a9. iContiguous_next Hnext 9.
+      iContiguous_next Hnext 10. }
     iFrame. iEpilogue "(HPC & Ha9 & Hr_t3)".
     iCombine "Ha9 Hprog_done" as "Hprog_done".
     (* iter *)
-    clear H4 H5 H6 H7 H8 H9 H10 H11 H12 H13 Hlt0 Hlt1 Hlt2 Hlt3 Hlt4 Hlt5 Hlt6 Hlt7 Hlt8.
+    clear H4 H5 H6 H7 H8 H9 H10 H11 H12 H13.
     do 5 iPrologue_pre. clear H4 H5 H6 H7.
     iDestruct "Hprog" as "[Hi1 Hprog]".
     iDestruct "Hprog" as "[Hi2 Hprog]".
@@ -760,86 +738,82 @@ Section stack_macros.
     iDestruct "Hprog" as "[Hi5 Hprog]".
     iDestruct "Hprog" as "[Hi6 Hprog]".
     iDestruct "Hregion" as (ws) "Hregion".
-    assert (a_first < a10)%Z as Hlt10;first middle_lt a9 10.
-    assert (a_first < a11)%Z as Hlt11; first middle_lt a10 11.
-    assert (a_first < a12)%Z as Hlt12; first middle_lt a11 12.
-    assert (a_first < a13)%Z as Hlt13; first middle_lt a12 13.
-    assert (a_first < a14)%Z as Hlt14; first middle_lt a13 14.
-    assert (a_first < a15)%Z as Hlt15; first middle_lt a14 15.
     iApply (mclear_iter_spec a10 a11 a12 a13 a14 a15 b_r e_r b_r _
                         0 p p' g b e r_t4 r_t1 r_t5 r_t6 r_t2 r_t3 _ p_r p_r' g_r
               with "[-]"); auto.
-    - split; [|(split; [|(split; [|(split; [|split])])])]; [iCorrectPC 11|iCorrectPC 12|iCorrectPC 13|iCorrectPC 14|iCorrectPC 15|iCorrectPC 16].
-    - repeat split;[apply Hnext with 11; auto|apply Hnext with 12; auto|
-                    apply Hnext with 13; auto|apply Hnext with 14; auto|apply Hnext with 15; auto].
+    - repeat apply conj; iCorrectPC a_first a'.
+    - repeat split; solve [
+        iContiguous_next Hnext 11; auto
+      | iContiguous_next Hnext 12; auto
+      | iContiguous_next Hnext 13; auto
+      | iContiguous_next Hnext 14; auto
+      | iContiguous_next Hnext 15; auto ].
     - (* rewrite Z.add_0_r. intros Hle. *)
-      rewrite /withinBounds.
-      apply andb_true_intro.
-      split; apply Z.leb_le; [lia|congruence].
+      rewrite /withinBounds. intro.
+      rewrite andb_true_iff Z.leb_le Z.ltb_lt. lia.
     - apply addr_add_0.
     - rewrite Z.add_0_r -Hb_r.
-      iFrame. rewrite Hb_r /=; iFrame. 
-      iSplitL "Hr_t6". iNext. iExists w6. iFrame. 
+      iFrame. rewrite Hb_r /=; iFrame.
+      iSplitL "Hr_t6". iNext. iExists w6. iFrame.
       iSplitR; auto.
-      iNext. rewrite -Hb_r. 
-      iIntros "(HPC & Hbe & Hr_t4 & Hr_t3 & Ha11 & Ha12 & Ha13 & Ha14 & 
+      iNext. rewrite -Hb_r.
+      iIntros "(HPC & Hbe & Hr_t4 & Hr_t3 & Ha11 & Ha12 & Ha13 & Ha14 &
       Ha9 & Hr_t5 & Hr_t1 & Ha10 & Hr_t2 & Hr_t6)".
-      iCombine "Ha9 Ha10 Ha11 Ha12 Ha13 Ha14 Hprog_done" as "Hprog_done". 
+      iCombine "Ha9 Ha10 Ha11 Ha12 Ha13 Ha14 Hprog_done" as "Hprog_done".
       iDestruct "Hr_t4" as (a_r0) "Hr_t4".
       iDestruct "Hr_t1" as (z0) "Hr_t1".
       iPrologue "Hprog".
       assert (a16 = a_end)%a as Ha16.
-      { simpl in Hjnz_off. 
+      { simpl in Hjnz_off.
         destruct Hjnz_off as (Ha16 & Ha16' & Hend).
-        by inversion Hend. 
-      } 
-      destruct a as [_ | a17 a]; inversion Hlen. 
-      assert (a_first < a16)%Z as Hlt16; first middle_lt a15 16. 
+        by inversion Hend.
+      }
+      destruct a as [_ | a17 a]; inversion Hlen.
       iApply (wp_move_success_z _ _ _ _ _ a16 a17 _ r_t4 _ 0 with "[HPC Hi Hr_t4]");
-        first apply move_z_i; first apply Hfl1; first iCorrectPC 17; auto. 
-      { apply Hnext with 17; auto. }
+        first apply move_z_i; first apply Hfl1;
+        first iCorrectPC a_first a'; auto.
+      { iContiguous_next Hnext 17; auto. }
       { rewrite Ha16. destruct p; iFrame. contradiction. }
       iEpilogue "(HPC & Ha16 & Hr_t4)".
       (* move r_t1 0 *)
       iPrologue "Hprog".
-      assert (a_first < a17)%Z as Hlt17; first middle_lt a16 17. 
       iApply (wp_move_success_z _ _ _ _ _ a17 a18 _ r_t1 _ 0 with "[HPC Hi Hr_t1]");
-        first apply move_z_i; first apply Hfl1; first iCorrectPC 18; auto.
-      { apply Hnext with 18; auto. }
+        first apply move_z_i; first apply Hfl1;
+        first iCorrectPC a_first a'; auto.
+      { iContiguous_next Hnext 18. }
       iFrame. iEpilogue "(HPC & Ha17 & Hr_t1)".
       (* move r_t2 0 *)
       iPrologue "Hprog".
-      assert (a_first < a18)%Z as Hlt18; first middle_lt a17 18. 
       iApply (wp_move_success_z _ _ _ _ _ a18 a19 _ r_t2 _ 0 with "[HPC Hi Hr_t2]");
-        first apply move_z_i; first apply Hfl1; first iCorrectPC 19; auto.
-      { apply Hnext with 19; auto. }
+        first apply move_z_i; first apply Hfl1;
+        first iCorrectPC a_first a'; auto.
+      { iContiguous_next Hnext 19. }
       iFrame. iEpilogue "(HPC & Ha18 & Hr_t2)".
       (* move r_t3 0 *)
       iPrologue "Hprog".
-      assert (a_first < a19)%Z as Hlt19; first middle_lt a18 19. 
       iApply (wp_move_success_z _ _ _ _ _ a19 a20 _ r_t3 _ 0 with "[HPC Hi Hr_t3]");
-        first apply move_z_i; first apply Hfl1; first iCorrectPC 20; auto.
-      { apply Hnext with 20; auto. }
+        first apply move_z_i; first apply Hfl1;
+        first iCorrectPC a_first a'; auto.
+      { iContiguous_next Hnext 20. }
       iFrame. iEpilogue "(HPC & Ha19 & Hr_t3)".
       (* move r_t5 0 *)
       iPrologue "Hprog".
-      assert (a_first < a20)%Z as Hlt20; first middle_lt a19 20. 
       iApply (wp_move_success_z _ _ _ _ _ a20 a21 _ r_t5 _ 0 with "[HPC Hi Hr_t5]");
-        first apply move_z_i; first apply Hfl1; first iCorrectPC 21; auto.
-      { apply Hnext with 21; auto. }
+        first apply move_z_i; first apply Hfl1;
+        first iCorrectPC a_first a'; auto.
+      { iContiguous_next Hnext 21. }
       iFrame. iEpilogue "(HPC & Ha20 & Hr_t5)".
       (* move r_t6 0 *)
       iPrologue "Hprog".
-      assert (a_first < a21)%Z as Hlt21; first middle_lt a20 21. 
       iApply (wp_move_success_z _ _ _ _ _ a21 a' _ r_t6 _ 0 with "[HPC Hi Hr_t6]");
-        first apply move_z_i; first apply Hfl1; first iCorrectPC 22; auto.
-      { inversion Ha_last. auto. }
+        first apply move_z_i; first apply Hfl1;
+        first iCorrectPC a_first a'; auto.
+      { eapply contiguous_between_last. eapply Hnext. reflexivity. }
       iFrame. iEpilogue "(HPC & Ha21 & Hr_t6)".
       iApply "Hφ".
       iDestruct "Hprog_done" as "(Ha_iter & Ha10 & Ha12 & Ha11 & Ha13 & Ha14 & Ha15 & Ha8 & Ha7
       & Ha6 & Ha5 & Ha4 & Ha3 & Ha2 & Ha1 & Ha0 & Ha_first)".
-      iFrame. Unshelve. exact 0. exact 0. apply w1. apply w1. 
+      iFrame. Unshelve. exact 0. exact 0. apply w1. apply w1.
   Qed.        (* ??? *)
-            
-         
-End stack_macros. 
+
+End stack_macros.
