theories/ftlr/Load.v
@@ -68,8 +68,8 @@ Section fundamental.
       apply reg_eq_sym in n. 
       iDestruct ("Hreg" $! src n) as "Hvsrc". 
       rewrite /RegLocate Hsomesrc.
-      iDestruct (read_allowed_inv _ a0 with "Hvsrc") as "Hconds"; auto; 
-        first (split; by apply Z.leb_le).        
+      iDestruct (read_allowed_inv _ a0 with "Hvsrc") as "Hconds"; auto;
+        first (split; [by apply Z.leb_le | by apply Z.ltb_lt]).
       (* Each condition in Hconds take a step in similar fashion *)
       destruct (decide (a = a0)).
       {
@@ -289,8 +289,8 @@ Section fundamental.
       iAssert ((fixpoint interp1) _ (inr (p0, l, a2, a1, a0))) as "#Hvsrc".
       { apply reg_eq_sym in n0. iDestruct ("Hreg" $! src n0) as "Hvsrc".
         rewrite /RegLocate Hsomesrc /=. by iApply "Hvsrc". }
-      iDestruct (read_allowed_inv _ a0 with "Hvsrc") as "Hconds"; auto; 
-        first (split; by apply Z.leb_le).
+      iDestruct (read_allowed_inv _ a0 with "Hvsrc") as "Hconds"; auto;
+        first (split; [by apply Z.leb_le | by apply Z.ltb_lt]).
       (* Each condition in Hconds take a step in similar fashion *)
       iAssert ((∃ w' p'', ▷ ((if (a0 =? a)%a then emp else a0 ↦ₐ[p''] w') -∗ open_region a W)
                             ∗ (if (a0 =? a)%a then emp else ▷ a0 ↦ₐ[p''] w')
